books/kestrel/utilities/fixbytes/defbytelist-tests.lisp
@@ -19,38 +19,38 @@
 ; test successful calls with default options:
 
 (must-succeed*
- (fty::defbyte 8)
- (fty::defbytelist ubyte8)
+ (fty::defbyte ubyte8 8)
+ (fty::defbytelist ubyte8-list ubyte8)
  (assert! (function-symbolp 'ubyte8-list-p (w state)))
  (assert! (function-symbolp 'ubyte8-list-fix$inline (w state)))
  (assert! (function-symbolp 'ubyte8-list-equiv$inline (w state))))
 
 (must-succeed*
- (fty::defbyte 16 :type word)
- (fty::defbytelist word)
+ (fty::defbyte word 16)
+ (fty::defbytelist word-list word)
  (assert! (function-symbolp 'word-list-p (w state)))
  (assert! (function-symbolp 'word-list-fix$inline (w state)))
  (assert! (function-symbolp 'word-list-equiv$inline (w state))))
 
 (must-succeed*
- (fty::defbyte 1 :signed t)
- (fty::defbytelist sbyte1)
+ (fty::defbyte sbyte1 1 :signed t)
+ (fty::defbytelist sbyte1-list sbyte1)
  (assert! (function-symbolp 'sbyte1-list-p (w state)))
  (assert! (function-symbolp 'sbyte1-list-fix$inline (w state)))
  (assert! (function-symbolp 'sbyte1-list-equiv$inline (w state))))
 
 (must-succeed*
  (defconst *size* 100)
- (fty::defbyte *size*)
- (fty::defbytelist ubyte100)
+ (fty::defbyte ubyte100 *size*)
+ (fty::defbytelist ubyte100-list ubyte100)
  (assert! (function-symbolp 'ubyte100-list-p (w state)))
  (assert! (function-symbolp 'ubyte100-list-fix$inline (w state)))
  (assert! (function-symbolp 'ubyte100-list-equiv$inline (w state))))
 
 (must-succeed*
  (define size () 50)
- (fty::defbyte (size) :type mybyte)
- (fty::defbytelist mybyte)
+ (fty::defbyte mybyte (size))
+ (fty::defbytelist mybyte-list mybyte)
  (assert! (function-symbolp 'mybyte-list-p (w state)))
  (assert! (function-symbolp 'mybyte-list-fix$inline (w state)))
  (assert! (function-symbolp 'mybyte-list-equiv$inline (w state))))
@@ -60,54 +60,60 @@
    (((size) => *))
    (local (defun size () 2))
    (defthm posp-of-size (posp (size))))
- (fty::defbyte (size) :type mybyte)
- (fty::defbytelist mybyte)
+ (fty::defbyte mybyte (size))
+ (fty::defbytelist mybyte-list mybyte)
  (assert! (function-symbolp 'mybyte-list-p (w state)))
  (assert! (function-symbolp 'mybyte-list-fix$inline (w state)))
  (assert! (function-symbolp 'mybyte-list-equiv$inline (w state))))
 
 ;;;;;;;;;;;;;;;;;;;;;;;;;;;;;;;;;;;;;;;;;;;;;;;;;;;;;;;;;;;;;;;;;;;;;;;;;;;;;;;;
 
-; test calls with a bad element type:
-
-(must-fail (fty::defbytelist "string"))
-
-(must-fail (fty::defbytelist (#\x 3/4)))
-
-(must-fail (fty::defbytelist not-even-a-fixtype))
-
-(must-fail (fty::defbytelist nat))
+; test the TYPE input:
 
 (must-succeed*
- (fty::defbyte 8 :type mybyte)
- (must-fail (fty::defbytelist mybyt)))
-
-;;;;;;;;;;;;;;;;;;;;;;;;;;;;;;;;;;;;;;;;;;;;;;;;;;;;;;;;;;;;;;;;;;;;;;;;;;;;;;;;
-
-; test the :TYPE input:
+ (fty::defbyte ubyte4 4)
+ (must-fail (fty::defbytelist #\A ubyte4)))
 
 (must-succeed*
- (fty::defbyte 4)
- (must-fail (fty::defbytelist ubyte4 :type #\A)))
-
-(must-succeed*
- (fty::defbyte 4)
- (fty::defbytelist ubyte4 :type nibbles)
+ (fty::defbyte ubyte4 4)
+ (fty::defbytelist nibbles ubyte4)
  (assert! (function-symbolp 'nibbles-p (w state)))
  (assert! (function-symbolp 'nibbles-fix$inline (w state)))
  (assert! (function-symbolp 'nibbles-equiv$inline (w state))))
 
 ;;;;;;;;;;;;;;;;;;;;;;;;;;;;;;;;;;;;;;;;;;;;;;;;;;;;;;;;;;;;;;;;;;;;;;;;;;;;;;;;
 
+; test the BYTE input:
+
+(must-fail (fty::defbytelist byte-list "string"))
+
+(must-fail (fty::defbytelist byte-list (#\x 3/4)))
+
+(must-fail (fty::defbytelist byte-list not-even-a-fixtype))
+
+(must-fail (fty::defbytelist byte-list nat))
+
+(must-succeed*
+ (fty::defbyte mybyte 8)
+ (must-fail (fty::defbytelist mybyte-list mybyt)))
+
+(must-succeed*
+ (fty::defbyte mybyte 5)
+ (fty::defbytelist mybyte-list mybyte)
+ (assert! (mybyte-list-p '(0 1 31)))
+ (assert! (not (mybyte-list-p '(32)))))
+
+;;;;;;;;;;;;;;;;;;;;;;;;;;;;;;;;;;;;;;;;;;;;;;;;;;;;;;;;;;;;;;;;;;;;;;;;;;;;;;;;
+
 ; test the :PRED input:
 
 (must-succeed*
- (fty::defbyte 4)
- (must-fail (fty::defbytelist ubyte4 :pred 888)))
+ (fty::defbyte byte 4)
+ (must-fail (fty::defbytelist bytes byte :pred 888)))
 
 (must-succeed*
- (fty::defbyte 4)
- (fty::defbytelist ubyte4 :pred nibblesp)
+ (fty::defbyte ubyte4 4)
+ (fty::defbytelist ubyte4-list ubyte4 :pred nibblesp)
  (assert! (function-symbolp 'nibblesp (w state)))
  (assert! (function-symbolp 'ubyte4-list-fix$inline (w state)))
  (assert! (function-symbolp 'ubyte4-list-equiv$inline (w state))))
@@ -117,12 +123,12 @@
 ; test the :FIX input:
 
 (must-succeed*
- (fty::defbyte 4)
- (must-fail (fty::defbytelist ubyte4 :fix #c(1 2))))
+ (fty::defbyte byte 4)
+ (must-fail (fty::defbytelist bytes byte :fix #c(1 2))))
 
 (must-succeed*
- (fty::defbyte 4)
- (fty::defbytelist ubyte4 :fix nibfix)
+ (fty::defbyte ubyte4 4)
+ (fty::defbytelist ubyte4-list ubyte4 :fix nibfix)
  (assert! (function-symbolp 'ubyte4-list-p (w state)))
  (assert! (function-symbolp 'nibfix$inline (w state)))
  (assert! (function-symbolp 'ubyte4-list-equiv$inline (w state))))
@@ -132,12 +138,12 @@
 ; test the :EQUIV input:
 
 (must-succeed*
- (fty::defbyte 4)
- (must-fail (fty::defbytelist ubyte4 :equiv (1 1 1))))
+ (fty::defbyte ubyte4 4)
+ (must-fail (fty::defbytelist ubyte4-list ubyte4 :equiv (1 1 1))))
 
 (must-succeed*
- (fty::defbyte 4)
- (fty::defbytelist ubyte4 :equiv nibeq)
+ (fty::defbyte ubyte4 4)
+ (fty::defbytelist ubyte4-list ubyte4 :equiv nibeq)
  (assert! (function-symbolp 'ubyte4-list-p (w state)))
  (assert! (function-symbolp 'ubyte4-list-fix$inline (w state)))
  (assert! (function-symbolp 'nibeq$inline (w state))))
@@ -147,45 +153,45 @@
 ; test the :PARENTS input:
 
 (must-succeed*
- (fty::defbyte 4)
- (must-fail (fty::defbytelist ubyte4 :parents one)))
+ (fty::defbyte byte 4)
+ (must-fail (fty::defbytelist byte-list byte :parents one)))
 
 (must-succeed*
- (fty::defbyte 4)
- (fty::defbytelist ubyte4 :parents nil))
+ (fty::defbyte byte 4)
+ (fty::defbytelist byte-list byte :parents nil))
 
 (must-succeed*
- (fty::defbyte 4)
- (fty::defbytelist ubyte4 :parents (this that)))
+ (fty::defbyte byte 4)
+ (fty::defbytelist byte-list byte :parents (this that)))
 
 ;;;;;;;;;;;;;;;;;;;;;;;;;;;;;;;;;;;;;;;;;;;;;;;;;;;;;;;;;;;;;;;;;;;;;;;;;;;;;;;;
 
 ; test the :SHORT input:
 
 (must-succeed*
- (fty::defbyte 4)
- (must-fail (fty::defbytelist ubyte4 :short #\s)))
+ (fty::defbyte byte 4)
+ (must-fail (fty::defbytelist bytes byte :short #\s)))
 
 (must-succeed*
- (fty::defbyte 4)
- (fty::defbytelist ubyte4 :short "Short doc."))
+ (fty::defbyte byte 4)
+ (fty::defbytelist bytes byte :short "Short doc."))
 
 (must-succeed*
- (fty::defbyte 4)
- (fty::defbytelist ubyte4 :short (concatenate 'string "Short" " " "doc.")))
+ (fty::defbyte byte 4)
+ (fty::defbytelist bytes byte :short (concatenate 'string "Short" " " "doc.")))
 
 ;;;;;;;;;;;;;;;;;;;;;;;;;;;;;;;;;;;;;;;;;;;;;;;;;;;;;;;;;;;;;;;;;;;;;;;;;;;;;;;;
 
 ; test the :LONG input:
 
 (must-succeed*
- (fty::defbyte 4)
- (must-fail (fty::defbytelist ubyte4 :long (#\t #\o #\p #\i #\c))))
+ (fty::defbyte byte 4)
+ (must-fail (fty::defbytelist bytes byte :long (#\t #\o #\p #\i #\c))))
 
 (must-succeed*
- (fty::defbyte 4)
- (fty::defbytelist ubyte4 :long "<p>More doc.</p>"))
+ (fty::defbyte byte 4)
+ (fty::defbytelist bytes byte :long "<p>More doc.</p>"))
 
 (must-succeed*
- (fty::defbyte 4)
- (fty::defbytelist ubyte4 :long (xdoc::topp "More doc.")))
+ (fty::defbyte byte 4)
+ (fty::defbytelist bytes byte :long (xdoc::topp "More doc.")))
