books/kestrel/ethereum/bytes.lisp
@@ -23,8 +23,7 @@
     Unless otherwise stated, in the documentation of our Ethereum model,
     the unqualified `byte' denotes an 8-bit byte."))
 
-(fty::defbyte 8
-  :type byte
+(fty::defbyte byte 8
   :pred bytep
   :parents (bytes)
   :short "Fixtype of bytes.")
@@ -54,7 +53,7 @@
     We use true lists of @(see bytes)
     to model byte arrays in our Ethereum model."))
 
-(fty::defbytelist byte
+(fty::defbytelist byte-list byte
   :pred byte-listp
   :parents (byte-arrays)
   :short "Fixtype of byte arrays.")
