books/kestrel/ethereum/nibbles.lisp
@@ -22,8 +22,7 @@
    "[YP:C] describes @($\\mathbb{Y}$) as the set of nibbles,
     which consist of 4 bits."))
 
-(fty::defbyte 4
-  :type nibble
+(fty::defbyte nibble 4
   :pred nibblep
   :parents (nibbles)
   :short "Fixtype of nibbles.")
@@ -45,7 +44,7 @@
     analogously to our model of
     <see topic='@(url byte-arrays)'>byte arrays</see>."))
 
-(fty::defbytelist nibble
+(fty::defbytelist nibble-list nibble
   :pred nibble-listp
   :parents (nibble-arrays)
   :short "Fixtype of nibble arrays.")
